finish LPR verification
- (modulo trivial syntactic cheats)

examples/lrat_checker/lratScript.sml
@@ -1,431 +1,17 @@
 (*
-   Verification of LRAT checker
+   Basic specification of an LRAT checker
+   - No optimizations
 *)
-open preamble miscTheory mlstringTheory;
+open preamble miscTheory mlstringTheory satSemTheory;
 
 val _ = new_theory "lrat";
 
-(*** Semantics ***
-
-  A literal is drawn from the sum 'a + 'a with the left projection being positive
-  and the right projection being negative
-
-  A clause is a set of literals (understood disjunctively)
-
-  A CNF is a set of clauses (understood conjunctively)
-
-  An assignment is a map from 'a to T/F
-
-  A clause is satisfied by an assignment if there is at least one of its literals assigned to true
-  A CNF is satisfied by an assignment if all its clauses are satisfied
-*)
-
-Type clause = ``:('a + 'a) set``;
-Type cnf = ``:'a clause set``;
-Type assignment = ``:'a -> bool``;
-
-val negate_literal_def = Define`
-  negate_literal l=
-  case l of
-    INL x => INR x
-  | INR x => INL x`
-
-val satisfies_literal_def = Define`
-  satisfies_literal (w:'a assignment) l ⇔
-  case l of
-    INL x => w x
-  | INR x => ¬w x`
-
-val satisfies_clause_def = Define`
-  satisfies_clause (w:'a assignment) (C:'a clause) ⇔
-  ∃l. l ∈ C ∧ satisfies_literal w l`
-
-val satisfies_def = Define`
-  satisfies (w:'a assignment) (fml:'a cnf) ⇔
-  ∀C. C ∈ fml ⇒ satisfies_clause w C`
-
-val satisfiable_def = Define`
-  satisfiable fml ⇔ ∃w. satisfies w fml`
-
-val unsatisfiable_def = Define`
-  unsatisfiable fml ⇔ ¬satisfiable fml`
-
-(*** Proofs about the semantics ***)
-
-(* General stuff about satisfiability *)
-
-(* Empty clauses are unsat *)
-Theorem empty_clause_imp_unsatisfiable:
-  {} ∈ fml ⇒
-  unsatisfiable fml
-Proof
-  rw[unsatisfiable_def,satisfiable_def,satisfies_def,satisfies_clause_def]>>
-  asm_exists_tac>>fs[]
-QED
-
-Theorem negate_negate[simp]:
-  negate_literal(negate_literal l) = l
-Proof
-  Cases_on`l`>>fs[negate_literal_def]
-QED
-
-(* l , -l are duals *)
-Theorem satisfies_literal_exclusive:
-  (satisfies_literal w l ⇔  ¬satisfies_literal w (negate_literal l))
-Proof
-  rw[EQ_IMP_THM,satisfies_literal_def]>>
-  every_case_tac>>fs[negate_literal_def]>>
-  rfs[]
-QED
-
-Theorem unsat_negate_satisfies_literal:
-  unsatisfiable ({negate_literal l} INSERT fml) ∧
-  satisfies w fml ⇒
-  satisfies_literal w l
-Proof
-  rw[unsatisfiable_def,satisfies_def,satisfiable_def]>>
-  first_x_assum(qspec_then`w` assume_tac)>>
-  fs[]
-  >-
-    (rw[]>>fs[satisfies_clause_def]>>
-    metis_tac[satisfies_literal_exclusive])
-  >>
-    metis_tac[]
-QED
-
-Theorem satisfies_clause_INSERT:
-  satisfies_clause w (l INSERT C) ⇔ satisfies_literal w l ∨ satisfies_clause w C
-Proof
-  rw[satisfies_clause_def]>>
-  metis_tac[]
-QED
-
-
-Theorem satisfies_INSERT:
-  satisfies w (C INSERT fml) ⇔ satisfies_clause w C ∧ satisfies w fml
-Proof
-  rw[satisfies_def]>>
-  metis_tac[]
-QED
-
-Theorem satisfies_SUBSET:
-  fml' ⊆ fml ⇒
-  satisfies w fml ⇒ satisfies w fml'
-Proof
-  rw[satisfies_def]>>
-  metis_tac[SUBSET_DEF]
-QED
-
-Theorem satisfiable_SUBSET:
-  fml' ⊆ fml ⇒
-  satisfiable fml ⇒ satisfiable fml'
-Proof
-  fs[satisfiable_def]>>
-  metis_tac[satisfies_SUBSET]
-QED
-
-Theorem satisfies_union:
-  satisfies w (A ∪ B) ⇔ satisfies w A ∧ satisfies w B
-Proof
-  rw[satisfies_def]>>
-  metis_tac[]
-QED
-
-Theorem satisfiable_DIFF:
-  satisfiable fml ⇒
-  satisfiable (fml DIFF clauses)
-Proof
-  fs[satisfiable_def,satisfies_def]>>
-  metis_tac[]
-QED
-
-Theorem sing_satisfies_literal:
-  {l} ∈ fml ∧
-  satisfies w fml ⇒
-  satisfies_literal w l
-Proof
-  rw[satisfies_def]>>
-  first_x_assum drule>>
-  fs[satisfies_clause_def]
-QED
-
-Theorem satisfies_clause_union:
-  satisfies_clause w (A ∪ B) ⇔ satisfies_clause w A ∨ satisfies_clause w B
-Proof
-  fs[satisfies_clause_def]>>
-  metis_tac[]
-QED
-
-Theorem satisfies_clause_SUBSET:
-  C ⊆ C' ∧
-  satisfies_clause w C ⇒ satisfies_clause w C'
-Proof
-  rw[satisfies_clause_def]>>
-  metis_tac[SUBSET_DEF]
-QED
-
-Theorem UNION_INSERT_EQ:
-  A ∪ (B INSERT C) = B INSERT (A ∪ C)
-Proof
-  fs[EXTENSION]>>metis_tac[]
-QED
-
-(* Definition of asymmetric tautologies *)
-val asymmetric_tautology_def = Define`
-  asymmetric_tautology fml C ⇔
-  unsatisfiable (fml ∪ (IMAGE (λl. {negate_literal l}) C))`
-
-Theorem list_unsat_negate_satisfies_literal:
-  ∀ls.
-  unsatisfiable (fml ∪ (IMAGE (λl. {negate_literal l}) C)) ∧
-  satisfies w fml ⇒
-  satisfies_clause w C
-Proof
-  rw[unsatisfiable_def,satisfiable_def,satisfies_union]>>
-  first_x_assum(qspec_then`w` assume_tac)>>
-  rfs[]>>
-  fs[satisfies_def]>>rw[]>>fs[satisfies_clause_def]>>
-  metis_tac[satisfies_literal_exclusive]
-QED
-
-Theorem asymmetric_tautology_satisfies:
-  ∀C fml.
-  asymmetric_tautology fml C ⇒
-  satisfies w fml ⇒
-  satisfies w (C INSERT fml)
-Proof
-  rw[asymmetric_tautology_def]>>
-  drule list_unsat_negate_satisfies_literal>>
-  disch_then drule>>
-  metis_tac[satisfies_INSERT]
-QED
-
-Theorem asymmetric_tautology_satisfiable:
-  ∀C fml.
-  asymmetric_tautology fml C ⇒
-  satisfiable fml ⇒
-  satisfiable (C INSERT fml)
-Proof
-  rw[satisfiable_def]>>
-  metis_tac[asymmetric_tautology_satisfies]
-QED
-
-Theorem asymmetric_tautology_set_satisfies:
-  ∀Cs fml.
-  (∀C. C ∈ Cs ⇒ asymmetric_tautology fml C) ⇒
-  satisfies w fml ⇒
-  satisfies w (Cs ∪ fml)
-Proof
-  rw[satisfies_union]>>
-  rw[satisfies_def]>>
-  first_x_assum drule>>
-  strip_tac>>
-  drule asymmetric_tautology_satisfies>>
-  disch_then drule>>
-  simp[satisfies_INSERT]
-QED
-
-Theorem tautology_asymmetric_tautology:
-  l ∈ C ∧ negate_literal l ∈ C
-  ⇒
-  asymmetric_tautology fml C
-Proof
-  rw[asymmetric_tautology_def,unsatisfiable_def,satisfiable_def,satisfies_def,MEM_MAP]>>
-  Cases_on`satisfies_literal w l`
-  >-
-    (qexists_tac`{negate_literal l}`>>fs[satisfies_clause_def]>>
-    metis_tac[satisfies_literal_exclusive])
-  >>
-    qexists_tac`{l}`>>fs[satisfies_clause_def]>>
-    DISJ2_TAC>>
-    qexists_tac`negate_literal l`>>simp[]
-QED
-
-val delete_literal_def = Define`
-  delete_literal l (C:'a clause) = C DIFF {l}`
-
-Theorem delete_literal_preserves_satisfies_clause_imp:
-  satisfies_clause w (delete_literal (negate_literal l) C) ⇒
-  satisfies_clause w C
-Proof
-  fs[delete_literal_def,satisfies_clause_def]>>
-  metis_tac[]
-QED
-
-Theorem delete_literal_preserves_satisfies_clause:
-  satisfies_literal w l ⇒
-  (satisfies_clause w C ⇔ satisfies_clause w (delete_literal (negate_literal l) C))
-Proof
-  rw[EQ_IMP_THM]
-  >- (
-    fs[delete_literal_def,satisfies_clause_def]>>
-    metis_tac[satisfies_literal_exclusive]
-  )
-  >>
-    fs[delete_literal_def,satisfies_clause_def]>>
-    metis_tac[]
-QED
-
-Theorem delete_unit_preserves_satisfies:
-  {l} ∈ fml ⇒
-  (satisfies w (C INSERT fml) ⇔ satisfies w ((delete_literal (negate_literal l) C) INSERT fml))
-Proof
-  fs[satisfies_INSERT]>>
-  metis_tac[delete_literal_preserves_satisfies_clause,sing_satisfies_literal]
-QED
-
-Theorem delete_unit_preserves_satisfiable:
-  {l} ∈ fml ⇒
-  (satisfiable (C INSERT fml) ⇔ satisfiable ((delete_literal (negate_literal l) C) INSERT fml))
-Proof
-  fs[satisfiable_def]>>
-  metis_tac[delete_unit_preserves_satisfies]
-QED
-
-(* Definition of resolution asymmetric tautology *)
-val resolution_asymmetric_tautology_def = Define`
-  resolution_asymmetric_tautology fml C ⇔
-  (asymmetric_tautology fml C ∨
-  ∃l. l ∈ C ∧
-  ∀D. D ∈ fml ∧ negate_literal l ∈ D ⇒
-    asymmetric_tautology fml (C ∪ delete_literal (negate_literal l) D))`
-
-(* soundness of resolution step *)
 (*
-Theorem resolution_sound:
-  l ≠ 0 ∧ (l::xs) ∈ fml ∧ ((-l)::ys) ∈ fml ⇒
-  (satisfies w fml ⇔ satisfies w ((xs++ys) INSERT fml))
-Proof
-  simp[EQ_IMP_THM]>>strip_tac>>strip_tac
-  >- (
-    rw[satisfies_INSERT]>>
-    fs[satisfies_def]>>
-    first_assum drule>>
-    first_x_assum(qspec_then `l::xs` mp_tac)>>fs[]>>
-    rw[satisfies_clause_def,MEM_FILTER]>>
-    metis_tac[satisfies_literal_exclusive])
-  >>
-    match_mp_tac satisfies_SUBSET>>
-    fs[SUBSET_DEF]
-QED
+  Bridging implementation and semantics
 
-Theorem resolution_sound1:
-  l ≠ 0 ∧ xs ∈ fml ∧ ys ∈ fml ∧
-  MEM l xs ∧ MEM (-l) ys ⇒
-  (satisfies w fml ⇔ satisfies w ((xs++delete_literal (-l) ys) INSERT fml))
-Proof
-  simp[EQ_IMP_THM]>>strip_tac>>strip_tac
-  >- (
-    rw[satisfies_INSERT]>>
-    fs[satisfies_def]>>
-    first_assum drule>>
-    first_x_assum(qspec_then `xs` mp_tac)>>fs[]>>
-    rw[satisfies_clause_def]>>
-    metis_tac[satisfies_literal_exclusive])
-  >>
-    match_mp_tac satisfies_SUBSET>>
-    fs[SUBSET_DEF]
-QED
-*)
+  Clauses are lists of integers where positive (>0) integers map to INL and negative (<0) map to INR
 
-val flip_literal_def = Define`
-  flip_literal l (w:'a assignment) =
-  case l of
-    INL x =>
-    λv. if v = x then ¬w x else w v
-  | INR x =>
-    λv. if v = x then ¬w x else w v`
-
-Theorem flip_literal_eq_neg:
-  flip_literal l w = flip_literal (negate_literal l) w
-Proof
-  simp[flip_literal_def]>>
-  TOP_CASE_TAC>>fs[negate_literal_def]
-QED
-
-Theorem flip_literal_flips:
-  (satisfies_literal w l ⇔ ¬(satisfies_literal (flip_literal l w) l))
-Proof
-  rw[satisfies_literal_def,flip_literal_def]>>
-  TOP_CASE_TAC>>fs[]
-QED
-
-Theorem flip_literal_unaffected:
-  satisfies_literal w l ∧
-  satisfies_clause w C ∧ l ∉ C ⇒
-  satisfies_clause (flip_literal l w ) C
-Proof
-  rw[satisfies_clause_def,satisfies_literal_def]>>
-  asm_exists_tac>>fs[]>>rw[]>>fs[]>>
-  every_case_tac>>fs[flip_literal_def]>>
-  metis_tac[]
-QED
-
-Theorem resolution_asymmetric_tautology_satisfiable:
-  ∀C fml w.
-  resolution_asymmetric_tautology fml C ⇒
-  satisfiable fml ⇒
-  satisfiable (C INSERT fml)
-Proof
-  rw[resolution_asymmetric_tautology_def]
-  >-
-    metis_tac[asymmetric_tautology_satisfiable]
-  >>
-  fs[satisfiable_def]>>
-  Cases_on`satisfies_clause w C`
-  >-
-    metis_tac[satisfies_INSERT]>>
-  qabbrev_tac`Ds = IMAGE (λD. C ∪ delete_literal (negate_literal l) D) { D | D ∈ fml ∧  (negate_literal l) ∈  D}`>>
-  `∀D. D ∈ Ds ⇒ asymmetric_tautology fml D` by
-    (rw[]>>fs[Abbr`Ds`])>>
-  drule asymmetric_tautology_set_satisfies >>
-  disch_then drule>>
-  strip_tac>>
-  fs[satisfies_union]>>
-  qabbrev_tac`w' = flip_literal l w`>>
-  qexists_tac`w'` >> rw[satisfies_INSERT]
-  >- (
-    `satisfies_literal w' l` by
-      (simp[Abbr`w'`]>>
-      metis_tac[flip_literal_flips,satisfies_clause_def])>>
-    metis_tac[satisfies_clause_def])
-  >>
-    `fml = { D | D ∈ fml ∧ ¬(negate_literal l ∈  D)} ∪ { D | D ∈ fml ∧ (negate_literal l ∈  D)}` by
-      (simp[EXTENSION]>>
-      metis_tac[])>>
-    pop_assum SUBST1_TAC>>
-    rw[satisfies_union]
-    >- (
-      fs[satisfies_def]>>rw[]>>
-      fs[Abbr`w'`]>>
-      simp[Once flip_literal_eq_neg]>>
-      match_mp_tac flip_literal_unaffected>>
-      metis_tac[satisfies_literal_exclusive,satisfies_clause_def])
-    >>
-      fs[satisfies_def]>>rw[]>>
-      `C ∪ delete_literal (negate_literal l) C' ∈ Ds` by
-        (fs[Abbr`Ds`]>>
-        qexists_tac`C'`>>fs[])>>
-      first_x_assum drule>> disch_then kall_tac>>
-      first_x_assum drule>>
-      simp[satisfies_clause_union]>>
-      strip_tac>>
-      `satisfies_clause w' (delete_literal (negate_literal l) C')` by
-        (simp[Abbr`w'`]>>
-        simp[Once flip_literal_eq_neg]>>
-        match_mp_tac flip_literal_unaffected>>
-        fs[delete_literal_def]>>
-        metis_tac[satisfies_literal_exclusive,satisfies_clause_def])>>
-      metis_tac[delete_literal_preserves_satisfies_clause_imp]
-QED
-
-(* Bridging implementation and semantics
-
-  Clauses are lists of integers
-
-  where positive (>0) integers map to INL and negative (<0) map to INR
-
-  In the implementation clauses are restricted to be SORTED by ≤ (i.e. no duplicates)
+  In implementation, clauses must not contain 0
 *)
 Type lit = ``:int``;
 Type cclause = ``:lit list``;
@@ -466,75 +52,35 @@ val interp_cclause_def = Define`
   interp_cclause (ls:cclause) =
   IMAGE interp_lit (set ls DIFF {0})`
 
-(*
-Theorem interp_cclause_eq:
-  interp_cclause ls =
-  {INL n | n ≠ 0 ∧ MEM (&n) ls} ∪ {INR n | n ≠ 0 ∧ MEM (-&n) ls}
-Proof
-  rw[EXTENSION,interp_cclause_def,EQ_IMP_THM]>>
-  rw[]
-  >- intLib.ARITH_TAC
-  >-
-    (`&Num (ABS x') = x'` by intLib.ARITH_TAC>>
-    fs[])
-  >- intLib.ARITH_TAC
-  >-
-    (`-&Num (ABS x') = x'` by intLib.ARITH_TAC>>
-    fs[])
-  >>
-  HINT_EXISTS_TAC>>fs[]>>
-  pop_assum kall_tac>>
-  intLib.ARITH_TAC
-QED
-*)
-
 val interp_def = Define`
   interp (fml:ccnf) = IMAGE interp_cclause (values fml)`
 
-(*** Implementation ***)
+(* Implementation *)
 val _ = Datatype`
   lratstep =
     Delete (num list) (* Clauses to delete *)
-  | RAT num cclause (num list) ((num list) spt)`
-    (* RAT step:
-      RAT n p C i0 (ik id ~> ik)
-      n is the new id of the new clause C
-      p is the pivot (first element of C in the input)
+  | PR num cclause (cclause option) (num list) ((num list) spt)`
+    (* PR step:
+      PR n C wopt i0 (ik id ~> ik)
+      n is the new id of the clause C
+      wopt is a witnessing assignment (represented as a list of literals)
+        if w is NONE, then this reduces to RAT
       i0 is a list of clause IDs for the AT part
       ik is a sptree mapping clause IDs to their hints
     *)
 
 Type lrat = ``:lratstep list``
 
-val list_delete_def = Define`
-  list_delete cl fml = FOLDL (\a b. delete b a) fml cl`
-
-val sorted_mem_def = Define`
-  (sorted_mem [] (x:lit) = F) ∧
-  (sorted_mem (y::ys) x =
-  if x > y then
-    sorted_mem ys x
-  else x = y)`
-
 val delete_literals_def = Define`
   delete_literals (C:cclause) (D:cclause) =
-  FILTER (λx. ¬ sorted_mem D x) C`
-
-val sorted_insert_def = Define`
-  (sorted_insert l [] = [l]) ∧
-  (sorted_insert (l:lit) (x::xs) =
-    if l < x then
-      l::(x::xs)
-    else if l = x then
-      l::xs
-    else
-      x:: (sorted_insert l xs))`
+  FILTER (λx. ¬MEM x D) C`
 
 (*
-  Checking for asymmetric tautology via unit propagation using the given hints
-  NONE == Error
-  SOME (INL ()) == C is an AT
-  SOME (INR C) == hints were insufficient, but C is now extended with units
+  Checking for asymmetric tautology via unit propagation using the given hints.
+  Returns:
+  NONE => Error
+  SOME (INL ()) => C is an AT
+  SOME (INR C) => hints were insufficient, but C is now extended with units
 *)
 val is_AT_def = Define`
   (is_AT fml [] (C:cclause) = SOME (INR C)) ∧
@@ -544,65 +90,68 @@ val is_AT_def = Define`
   | SOME Ci =>
   case delete_literals Ci C of
     [] => SOME (INL ())
-  | [l] => is_AT fml is (sorted_insert (-l) C)
+  | [l] => is_AT fml is (-l :: C)
   | _ => NONE)`
 
-(* merge sorted lists *)
-val sorted_union_def = Define`
-  (sorted_union [] (rs:cclause) = rs) ∧
-  (sorted_union ls [] = ls) ∧
-  (sorted_union (l::ls) (r::rs) =
-    if l < r then
-      l :: sorted_union ls (r::rs)
-    else if l = r then
-      l :: sorted_union ls rs
-    else
-      r :: sorted_union (l::ls) rs)`
+(* Check if Ci overlaps with a list of assignments *)
+val check_overlap_def = Define`
+  (check_overlap Ci [] = F) ∧
+  (check_overlap Ci (a::as) =
+    (MEM a Ci ∨ check_overlap Ci as))`
 
-val sorted_delete_def = Define`
-  (sorted_delete p [] = []) ∧
-  (sorted_delete (p:lit) (x::xs) =
-    if p > x then x::(sorted_delete p xs)
-    else if p = x then sorted_delete p xs
-    else x::xs)`
+(* flips a clause/assignment.
+  for a clause, this yields its blocked assignment *)
+val flip_def = Define`
+  flip (C:cclause) = MAP (λi. -i) C`
 
-val find_tauto_def = Define`
-  (find_tauto p C [] = F) ∧
-  (find_tauto (p:int) C (c::cs) =
-    if c = -p then find_tauto p C cs
-    else
-      if sorted_mem C (-c) then T
-      else find_tauto p C cs
-  )`
-
-(*
-  Resolution Asymmetric Tautology
+(* Construct the overlapping assignment
+  { w ∪ negate (C) }
+  where w overrides everything in negate(C)
 *)
-val is_RAT_aux_def = Define`
-  (is_RAT_aux fml (p:int) C ik [] = T) ∧
-  (is_RAT_aux fml p C ik (iCi::iCs) =
-  case iCi of (i,Ci) =>
-    if sorted_mem Ci (-p)then
-      case lookup i ik of
-        NONE => F
-      | SOME is =>
-        case is of [] =>
-        (* Step 5.2: can be made more efficient *)
-          if find_tauto p C Ci then
-            is_RAT_aux fml p C ik iCs
-          else
-            F
-        | _ =>
-          (* Step 5.3-5.5 *)
-          if is_AT fml is (sorted_union C (sorted_delete (-p) Ci)) = SOME (INL ()) then
-            is_RAT_aux fml p C ik iCs
-          else
-            F
-    else
-      is_RAT_aux fml p C ik iCs)`
+val overlap_assignment_def = Define`
+  overlap_assignment w C =
+    w ++ flip (delete_literals C w)`
 
-val is_RAT_def = Define`
-  is_RAT fml p (C:cclause) i0 ik =
+(* The (L)RAT check (no witnesses) *)
+val check_RAT_def = Define`
+  check_RAT fml p C ik (i,Ci) =
+  (* Step 5.1: if Ci contains -p do work, else skip *)
+  if check_overlap Ci [-p] then
+    (* Lookup the hint *)
+    case lookup i ik of
+      NONE => F
+    | SOME is =>
+    case is of
+      (* Step 5.2: Ci is satisfied by p ∪ negate (C) *)
+      [] => check_overlap Ci (overlap_assignment [p] C)
+    | _ =>
+      (* Step 5.3-5.5: Otherwise, use full hints *)
+      is_AT fml is (C ++ (delete_literals Ci [-p])) = SOME (INL ())
+  else
+    T`
+
+(* The (L)PR check (witness given) *)
+val check_PR_def = Define`
+  check_PR fml p C w ik (i,Ci) =
+  (* Step 5.1: if Ci is touched by w do work, else skip *)
+  if check_overlap Ci (flip w) then
+    (* Lookup the hint *)
+    case lookup i ik of
+      NONE =>
+      (* Step 5.2.1: Ci is satisfied by w *)
+      check_overlap Ci w
+    | SOME is =>
+    case is of
+      (* Step 5.2.2: Ci is satisfied by w ∪ negate (C) *)
+      [] => check_overlap Ci (overlap_assignment w C)
+    | _ =>
+      (* Step 5.3-5.5: Otherwise use full hints *)
+      is_AT fml is (C ++ (delete_literals Ci (flip (overlap_assignment w C)))) = SOME (INL ())
+  else
+    T`
+
+val is_PR_def = Define`
+  is_PR fml p (C:cclause) wopt i0 ik =
   (* First, do the asymmetric tautology check *)
   case is_AT fml i0 C of
     NONE => F
@@ -610,20 +159,22 @@ val is_RAT_def = Define`
   | SOME (INR D) =>
   if p ≠ 0 then
     let iCs = toAList fml in
-      is_RAT_aux fml p D ik iCs
+    case wopt of
+      NONE => EVERY (check_RAT fml p D ik) iCs
+    | SOME w =>
+      ¬(check_overlap w (flip w)) ∧
+      EVERY (check_PR fml p D w ik) iCs
   else
      F`
 
 val check_lrat_step_def = Define`
   check_lrat_step step fml =
   case step of
-    Delete cl =>
-      SOME (list_delete cl fml)
-  | RAT n C i0 ik =>
+    Delete cl => SOME (FOLDL (\a b. delete b a) fml cl)
+  | PR n C w i0 ik =>
     let p = case C of [] => 0 | (x::xs) => x in
-    let C = QSORT $<= (FILTER (λx. x ≠ 0) C) in
-    if is_RAT fml p C i0 ik then
-      SOME (insert n C fml)
+    if is_PR fml p C w i0 ik
+    then SOME (insert n C fml)
     else NONE`
 
 val is_unsat_def = Define`
@@ -645,35 +196,13 @@ val check_lrat_unsat_def = Define`
     NONE => F
   | SOME fml' => is_unsat fml'`
 
+(* Proofs *)
 val wf_clause_def = Define`
-  wf_clause (C:cclause) ⇔ ¬ MEM 0 C ∧ SORTED $<= C`
+  wf_clause (C:cclause) ⇔ ¬ MEM 0 C`
 
 val wf_fml_def = Define`
   wf_fml (fml:ccnf) ⇔
   ∀C. C ∈ values fml ⇒ wf_clause C`
-
-Theorem sorted_mem_correct:
-  ∀ls.
-  wf_clause ls ⇒
-  sorted_mem ls x = MEM x ls
-Proof
-  simp[wf_clause_def]>>
-  Induct>>fs[sorted_mem_def]>>
-  Cases_on`ls`>>fs[sorted_mem_def]
-  >- intLib.ARITH_TAC>>
-  rw[]>>
-  fs[SORTED_DEF]>>
-  simp[EQ_IMP_THM]>>
-  rw[]>>fs[]>>
-  TRY( `F` by
-    (pop_assum kall_tac>>last_x_assum kall_tac>>
-    intLib.ARITH_TAC))
-  >-
-    (ntac 2 (pop_assum kall_tac)>>
-    intLib.ARITH_TAC)>>
-  EVERY_CASE_TAC>>
-  intLib.ARITH_TAC
-QED
 
 Theorem filter_unit_preserves_satisfies:
   ∀C.
@@ -717,8 +246,7 @@ Proof
   intLib.ARITH_TAC
 QED
 
-Theorem delete_literals_correct:
-  wf_clause C ∧ wf_clause D ⇒
+Theorem interp_cclause_delete_literals:
   interp_cclause (delete_literals C D) =
   interp_cclause C DIFF interp_cclause D
 Proof
@@ -726,66 +254,8 @@ Proof
   fs[interp_cclause_def]>>
   fs[EXTENSION]>>
   rw[EQ_IMP_THM]>>
-  fs[MEM_FILTER]
-  >- metis_tac[]
-  >-
-    (metis_tac[sorted_mem_correct,interp_lit_eq])>>
-  qexists_tac`x'`>>fs[sorted_mem_correct]>>
-  metis_tac[]
-QED
-
-Theorem wf_clause_cons:
-  wf_clause (x::y) ⇔
-  x ≠ 0 ∧
-  (y = [] ∨ x <= HD y ∧ wf_clause y)
-Proof
-  Cases_on`y`>>fs[wf_clause_def,EQ_IMP_THM,SORTED_DEF]
-QED
-
-Theorem sorted_insert_less:
-  ∀ls.
-  h' <= HD ls ∧ h' <= h ⇒
-  h' <= HD (sorted_insert h ls)
-Proof
-  Induct>>rw[sorted_insert_def]
-QED
-
-Theorem wf_clause_sorted_insert:
-  ∀C.
-  wf_clause C ∧ h ≠ 0 ⇒
-  wf_clause (sorted_insert h C)
-Proof
-  Induct>>fs[sorted_insert_def]
-  >-
-    simp[wf_clause_def]>>
-  rw[]
-  >-
-    fs[wf_clause_def,SORTED_DEF]>>
-  fs[wf_clause_cons,sorted_insert_def,wf_clause_def]
-  >-
-    intLib.ARITH_TAC
-  >>
-  DISJ2_TAC >> match_mp_tac sorted_insert_less>>
-  fs[]>>
-  intLib.ARITH_TAC
-QED
-
-Theorem set_sorted_insert:
-  ∀C. set (sorted_insert h C) = h INSERT set C
-Proof
-  Induct>>rw[sorted_insert_def]>>
-  rw[EXTENSION]>>
-  metis_tac[]
-QED
-
-Theorem interp_cclause_sorted_insert:
-  ∀C.
-  interp_cclause (sorted_insert h C) =
-  interp_cclause [h] ∪ interp_cclause C
-Proof
-  rw[]>>simp[interp_cclause_def,set_sorted_insert]>>
-  rw[]>>
-  metis_tac[INSERT_SING_UNION]
+  fs[MEM_FILTER]>>
+  metis_tac[interp_lit_eq]
 QED
 
 Theorem negate_literal_interp_lit:
@@ -804,153 +274,6 @@ Proof
   simp[interp_cclause_def]>>
   simp[negate_literal_interp_lit]
 QED
-
-(* is_AT is correct in the INL case *)
-Theorem is_AT_imp_asymmetric_tautology:
-  ∀is fml C.
-  wf_fml fml ∧ wf_clause C ⇒
-  is_AT fml is C = SOME (INL ()) ⇒
-    asymmetric_tautology (interp fml) (interp_cclause C)
-Proof
-  Induct>>fs[is_AT_def]>>
-  ntac 4 strip_tac>>
-  every_case_tac>>fs[]>>
-  `interp_cclause x DIFF interp_cclause C = interp_cclause (delete_literals x C)` by
-    (match_mp_tac (GSYM delete_literals_correct)>>
-    fs[wf_fml_def,values_def]>>metis_tac[])
-  >-
-    (fs[asymmetric_tautology_def]>>
-    qmatch_goalsub_abbrev_tac`unsatisfiable fml'`>>
-    `fml' = (interp_cclause x) INSERT fml'` by
-      (match_mp_tac (GSYM ABSORPTION_RWT)>>
-      fs[Abbr`fml'`,values_def,interp_def]>>
-      metis_tac[])>>
-    pop_assum SUBST1_TAC>>
-    match_mp_tac filter_unit_preserves_unsatisfiable>>
-    qexists_tac`interp_cclause C`>>rw[]
-    >-
-      fs[Abbr`fml'`]
-    >>
-    match_mp_tac empty_clause_imp_unsatisfiable>>
-    simp[interp_cclause_def])
-  >>
-    strip_tac>>
-    `wf_clause x` by
-      (fs[wf_fml_def,values_def]>>
-      metis_tac[])>>
-    `MEM h' (delete_literals x C)` by fs[]>>
-    `-h' ≠ 0` by
-      (fs[wf_clause_def,delete_literals_def,MEM_FILTER]>>
-      metis_tac[])>>
-    last_x_assum drule>>
-    disch_then (qspec_then`sorted_insert (-h') C` mp_tac)>>simp[]>>
-    impl_tac >-
-      metis_tac[wf_clause_sorted_insert]>>
-    simp[asymmetric_tautology_def]>>
-    rw[]>>fs[]>>
-    qmatch_goalsub_abbrev_tac`unsatisfiable fml'`>>
-    `(interp_cclause x) INSERT fml' = fml'` by
-      (match_mp_tac ABSORPTION_RWT>>
-      fs[Abbr`fml'`,values_def,interp_def]>>
-      metis_tac[])>>
-    pop_assum (SUBST1_TAC  o SYM)>>
-    match_mp_tac filter_unit_preserves_unsatisfiable>>
-    qexists_tac`interp_cclause C`>>rw[]
-    >-
-      simp[Abbr`fml'`]
-    >>
-      rfs[interp_cclause_sorted_insert, interp_cclause_negate_literal]>>
-      fs[Abbr`fml'`]>>
-      metis_tac[UNION_INSERT_EQ,INSERT_SING_UNION]
-QED
-
-Theorem satisfies_clause_DIFF:
-  satisfies_clause w C ∧
-  ¬satisfies_clause w D ⇒
-  satisfies_clause w (C DIFF D)
-Proof
-  fs[satisfies_clause_def]>>
-  metis_tac[]
-QED
-
-Theorem is_AT_imp_sat_preserving:
-  ∀is fml C D.
-  wf_fml fml ∧ wf_clause C ⇒
-  is_AT fml is C = SOME (INR D) ⇒
-  ∃E.
-    interp_cclause D = E ∪ interp_cclause C ∧
-    wf_clause D ∧
-    ∀w.
-    satisfies w (interp_cclause D INSERT interp fml) ⇒
-    satisfies w (interp_cclause C INSERT interp fml)
-Proof
-  Induct>>fs[is_AT_def]>>
-  rw[]
-  >-
-    (qexists_tac`{}`>>simp[])>>
-  every_case_tac>>fs[]>>
-  `interp_cclause x DIFF interp_cclause C = interp_cclause (delete_literals x C)` by
-    (match_mp_tac (GSYM delete_literals_correct)>>
-    fs[wf_fml_def,values_def]>>metis_tac[])>>
-  `wf_clause x` by
-    (fs[wf_fml_def,values_def]>>
-    metis_tac[])>>
-  `MEM h' (delete_literals x C)` by fs[]>>
-  `-h' ≠ 0` by
-    (fs[wf_clause_def,delete_literals_def,MEM_FILTER]>>
-    metis_tac[])>>
-  first_x_assum drule>>
-  disch_then(qspecl_then [`sorted_insert (-h') C`,`D`] mp_tac)>>simp[]>>
-  impl_tac >-
-    metis_tac[wf_clause_sorted_insert]>>
-  strip_tac>>
-  fs[interp_cclause_sorted_insert,UNION_ASSOC]>>
-  qexists_tac`E ∪ interp_cclause [-h']`>> simp[]>>
-  rw[]>>fs[]>>
-  qpat_x_assum` _ D = _` SUBST_ALL_TAC>>
-  first_x_assum drule>>
-  strip_tac>>
-  fs[satisfies_INSERT]>>
-  `satisfies_clause w (interp_cclause x)` by
-    (fs[satisfies_def,interp_def,values_def]>>
-    metis_tac[])>>
-  CCONTR_TAC >> fs[]>>
-  `interp_cclause x DIFF interp_cclause C = interp_cclause [h']` by
-    fs[]>>
-  `satisfies_clause w (interp_cclause [h'])` by
-    metis_tac[satisfies_clause_DIFF]>>
-  fs[satisfies_clause_union]>>
-  qpat_x_assum`h' ≠ 0` mp_tac>>
-  ntac 2 (qpat_x_assum`satisfies_clause w ( _ [_])` mp_tac)>>
-  rpt( pop_assum kall_tac)>>
-  rw[interp_cclause_def]>>
-  fs[satisfies_clause_def]>>
-  metis_tac[negate_literal_interp_lit,satisfies_literal_exclusive]
-QED
-
-(*
-Theorem find_exists_mem:
-  ∀ls. find_exists s ls ⇒ ∃k v. (k ∈ domain s ∧ MEM (k,v) ls)
-Proof
-  Induct>>fs[find_exists_def]>>Cases>>fs[]>>
-  rw[]>>fs[domain_lookup]>>metis_tac[]
-QED
-
-Theorem find_tauto_correct:
-  ∀C D.
-  find_tauto C D ⇒
-  ∃l. l ∈ interp_cclause C ∧ negate_literal l ∈ interp_cclause D
-Proof
-  Cases>>Cases>>rw[find_tauto_def]>>
-  drule find_exists_mem>>
-  rw[]>>fs[MEM_toAList]>>
-  fs[interp_cclause_def,domain_lookup]
-  >-
-    (qexists_tac`INL k`>>simp[negate_literal_def])
-  >>
-    qexists_tac`INR k`>>simp[negate_literal_def]
-QED
-*)
 
 Theorem interp_cclause_empty[simp]:
   interp_cclause [] = {}
@@ -972,282 +295,492 @@ Proof
 QED
 
 Theorem interp_cclause_cons:
-  interp_cclause (x::C) = interp_cclause [x] ∪ interp_cclause C
+  interp_cclause (h::C) =
+  interp_cclause [h] ∪ interp_cclause C
 Proof
-  metis_tac[CONS_APPEND,interp_cclause_append]
+  rw[interp_cclause_def]>>
+  metis_tac[INSERT_SING_UNION]
 QED
 
-val sorted_union_ind = fetch "-" "sorted_union_ind";
-
-Theorem transitive_leq[simp]:
-  transitive ($<= : int -> int -> bool)
+(* is_AT is correct in the INL case *)
+Theorem is_AT_imp_asymmetric_tautology:
+  ∀is fml C.
+  wf_fml fml ∧ wf_clause C ∧
+  is_AT fml is C = SOME (INL ()) ⇒
+    asymmetric_tautology (interp fml) (interp_cclause C)
 Proof
-  fs[transitive_def]>>
-  intLib.ARITH_TAC
-QED
-
-Theorem wf_clause_less:
-  p < h ∧ wf_clause (h::C) ⇒
-  interp_lit p ∉ interp_cclause (h::C)
-Proof
-  CCONTR_TAC>>fs[interp_cclause_def]>>
-  every_case_tac>>fs[wf_clause_def]
+  Induct>>fs[is_AT_def]>>
+  ntac 4 strip_tac>>
+  every_case_tac>>fs[]>>
+  `interp_cclause x DIFF interp_cclause C = interp_cclause (delete_literals x C)` by
+    fs[interp_cclause_delete_literals]
   >-
-    (rw[]>>
-    `p=h` by fs[interp_lit_eq]>>
-    intLib.ARITH_TAC)
+    (fs[asymmetric_tautology_def]>>
+    qmatch_goalsub_abbrev_tac`unsatisfiable fml'`>>
+    `fml' = (interp_cclause x) INSERT fml'` by
+      (match_mp_tac (GSYM ABSORPTION_RWT)>>
+      fs[Abbr`fml'`,values_def,interp_def]>>
+      metis_tac[])>>
+    pop_assum SUBST1_TAC>>
+    match_mp_tac filter_unit_preserves_unsatisfiable>>
+    qexists_tac`interp_cclause C`>>rw[]
+    >-
+      fs[Abbr`fml'`]
+    >>
+    match_mp_tac empty_clause_imp_unsatisfiable>>
+    simp[interp_cclause_def])
   >>
-    `p=x` by fs[interp_lit_eq]>>
-    qpat_x_assum`SORTED _ _` mp_tac>>
-    dep_rewrite.DEP_REWRITE_TAC [SORTED_EQ]>>
-    simp[]>>
-    `~(h ≤ p)` by intLib.ARITH_TAC>>
-    metis_tac[]
-QED
-
-Theorem interp_cclause_sorted_delete:
-  ∀C.
-  wf_clause C ⇒
-  interp_cclause (sorted_delete p C) =
-  delete_literal (interp_lit p) (interp_cclause C)
-Proof
-  Induct>>fs[sorted_delete_def,delete_literal_def]>>
-  rw[]>>fs[]>>
-  `wf_clause C'` by
-    fs[wf_clause_cons]>>fs[]
-  >-
-    (simp[Once interp_cclause_cons]>>
-    simp[Once interp_cclause_cons,SimpRHS]>>
-    rw[EXTENSION,EQ_IMP_THM]>>
-    fs[interp_cclause_def]>>
-    pop_assum mp_tac>>
-    IF_CASES_TAC>>rw[]>>
-    `p ≠ h` by
-      intLib.ARITH_TAC>>
-    metis_tac[interp_lit_eq])
-  >-
-    (simp[Once interp_cclause_cons]>>
-    simp[interp_cclause_def]>>rw[EXTENSION,EQ_IMP_THM]>>
-    metis_tac[])
-  >>
-    `p < h` by intLib.ARITH_TAC>>
-    drule wf_clause_less>>
-    rw[EXTENSION,EQ_IMP_THM]>>
-    rw[interp_cclause_def]>>fs[]>>
-    metis_tac[]
-QED
-
-Theorem interp_cclause_sorted_union:
-  ∀C D.
-  wf_clause C ∧ wf_clause D ⇒
-  interp_cclause (sorted_union C D) =
-  interp_cclause C ∪ interp_cclause D
-Proof
-  ho_match_mp_tac sorted_union_ind>>rw[sorted_union_def]>>
-  fs[]>>qpat_x_assum`_ ⇒ _` mp_tac>>
-  (impl_tac>- fs[wf_clause_cons])>> rw[]>>
-  simp[Once interp_cclause_cons]
-  >-
-    metis_tac[interp_cclause_cons,UNION_ASSOC]
-  >-
-    metis_tac[interp_cclause_cons,UNION_ASSOC,UNION_IDEMPOT,UNION_COMM]
-  >>
-    `interp_cclause (r::D) = interp_cclause [r] ∪ interp_cclause D` by
-      simp[Once interp_cclause_cons]>>
-    simp[]>>
-    simp[UNION_ASSOC]>>
-    metis_tac[UNION_COMM]
-QED
-
-Theorem MEM_sorted_delete:
-  ∀C.
-  MEM x (sorted_delete p C) ⇒
-  MEM x C
-Proof
-  Induct>>rw[sorted_delete_def]>>
-  metis_tac[]
-QED
-
-Theorem wf_clause_sorted_delete:
-  ∀C. wf_clause C ⇒
-  wf_clause (sorted_delete p C)
-Proof
-  Induct>>fs[sorted_delete_def,delete_literal_def]>>
-  rw[]>>fs[]>>
-  `wf_clause C'` by
-    fs[wf_clause_cons]>>fs[]>>
-  fs[Once wf_clause_cons]>>
-  simp[sorted_delete_def]>>
-  Cases_on`sorted_delete p C'`>>fs[wf_clause_def]>>
-  `MEM h' (sorted_delete p C')` by fs[]>>
-  drule MEM_sorted_delete>>
-  qpat_x_assum` SORTED _ (h'::t)` mp_tac>>
-  dep_rewrite.DEP_REWRITE_TAC[SORTED_EQ]>>
-  simp[]>>
-  Cases_on`C'`>>fs[]>>
-  qpat_x_assum`SORTED _ (_::_)` mp_tac>>
-  dep_rewrite.DEP_REWRITE_TAC[SORTED_EQ]>>
-  simp[]>>
-  metis_tac[integerTheory.INT_LE_TRANS]
-QED
-
-Theorem sorted_union_MEM:
-  ∀C D.
-  MEM x (sorted_union C D) ⇒
-  MEM x C ∨ MEM x D
-Proof
-  ho_match_mp_tac sorted_union_ind>>rw[sorted_union_def]>>
-  fs[]
-QED
-
-Theorem wf_clause_sorted_union:
-  ∀C D.
-  wf_clause C ∧ wf_clause D ⇒
-  wf_clause (sorted_union C D)
-Proof
-  ho_match_mp_tac sorted_union_ind>>rw[sorted_union_def]>>
-  fs[]>>qpat_x_assum`_ ⇒ _` mp_tac>>
-  (impl_tac>- fs[wf_clause_cons])>> rw[]>>
-  simp[Once wf_clause_cons]
-  >-
-    (fs[wf_clause_def]>> rw[]>>
-    Cases_on`sorted_union C (r::D)`>>fs[]>>
-    rpt(qpat_x_assum`SORTED _ (_::_)` mp_tac)>>
-    dep_rewrite.DEP_REWRITE_TAC [SORTED_EQ]>>
-    simp[]>>
-    `MEM h C ∨ MEM h (r::D)` by
-      fs[sorted_union_MEM]>>
-    fs[]>>
-    rw[]>>first_x_assum drule>>
-    intLib.ARITH_TAC)
-  >-
+  `wf_clause x` by
+    (fs[wf_fml_def,values_def]>>
+    metis_tac[])>>
+  `MEM h' (delete_literals x C)` by fs[]>>
+  `-h' ≠ 0` by
+    (fs[wf_clause_def,delete_literals_def,MEM_FILTER]>>
+    metis_tac[])>>
+  last_x_assum drule>>
+  disch_then (qspec_then`(-h')::C` mp_tac)>>simp[]>>
+  impl_tac >-
     (fs[wf_clause_def]>>
-    Cases_on`sorted_union C D`>>fs[]>>
-    rpt(qpat_x_assum`SORTED _ (_::_)` mp_tac)>>
-    dep_rewrite.DEP_REWRITE_TAC [SORTED_EQ]>>
-    simp[]>>
-    `MEM h C ∨ MEM h D` by fs[sorted_union_MEM]>>
-    fs[])
+    intLib.ARITH_TAC)>>
+  simp[asymmetric_tautology_def]>>
+  rw[]>>fs[]>>
+  qmatch_goalsub_abbrev_tac`unsatisfiable fml'`>>
+  `(interp_cclause x) INSERT fml' = fml'` by
+    (match_mp_tac ABSORPTION_RWT>>
+    fs[Abbr`fml'`,values_def,interp_def]>>
+    metis_tac[])>>
+  pop_assum (SUBST1_TAC  o SYM)>>
+  match_mp_tac filter_unit_preserves_unsatisfiable>>
+  qexists_tac`interp_cclause C`>>rw[]
+  >-
+    simp[Abbr`fml'`]
   >>
-    (fs[wf_clause_def]>> rw[]>>
-    Cases_on`sorted_union (l::C) D`>>fs[]>>
-    rpt(qpat_x_assum`SORTED _ (_::_)` mp_tac)>>
-    dep_rewrite.DEP_REWRITE_TAC [SORTED_EQ]>>
-    simp[]>>
-    `MEM h (l::C) ∨ MEM h D` by
-      fs[sorted_union_MEM]>>
-    fs[]
-    >-
-      (rw[]>>intLib.ARITH_TAC)>>
-    rw[]>>first_x_assum drule>>
-    intLib.ARITH_TAC)
+    fs[Abbr`fml'`]>>
+    pop_assum mp_tac>>
+    simp[Once interp_cclause_cons]>>
+    simp[interp_cclause_negate_literal]>>
+    metis_tac[UNION_INSERT_EQ,INSERT_SING_UNION]
 QED
 
-Theorem find_tauto_correct:
-  ∀ls p C.
-  wf_clause C ∧
-  find_tauto p C ls ⇒
-  ∃l. MEM l ls ∧ MEM (-l) C ∧ l ≠ -p
+Theorem satisfies_clause_DIFF:
+  satisfies_clause w C ∧
+  ¬satisfies_clause w D ⇒
+  satisfies_clause w (C DIFF D)
 Proof
-  Induct>>rw[find_tauto_def]>>
-  rfs[sorted_mem_correct]>>
+  fs[satisfies_clause_def]>>
   metis_tac[]
 QED
 
-Theorem is_RAT_aux_imp:
-  ∀iCs fml p C ik.
-  wf_fml fml ∧ wf_clause C ∧ EVERY wf_clause (MAP SND iCs) ∧ p ≠ 0 ⇒
-  is_RAT_aux fml p C ik iCs ⇒
-  ∀i Ci. MEM (i,Ci) iCs ∧ sorted_mem Ci (-p) ⇒
-    asymmetric_tautology (interp fml) (interp_cclause C ∪ interp_cclause (sorted_delete (-p) Ci))
+Theorem is_AT_imp_sat_implies:
+  ∀is fml C D.
+  wf_fml fml ∧ wf_clause C ⇒
+  is_AT fml is C = SOME (INR D) ⇒
+  ∃E.
+    interp_cclause D = E ∪ interp_cclause C ∧
+    wf_clause D ∧
+    sat_implies
+      (interp_cclause D INSERT interp fml)
+      (interp_cclause C INSERT interp fml)
 Proof
-  Induct>>Cases>>fs[is_RAT_aux_def]>>
-  ntac 4 strip_tac >>
-  reverse IF_CASES_TAC>>fs[]
+  Induct>>fs[is_AT_def]>>
+  rw[]
   >-
-    (* 5.1 *)
-    (strip_tac>>fs[PULL_FORALL,AND_IMP_INTRO]>>
-    rw[]>>first_x_assum match_mp_tac>>fs[]>>
-    metis_tac[])
-  >>
+    (qexists_tac`{}`>>simp[sat_implies_def])>>
+  every_case_tac>>fs[]>>
+  `interp_cclause x DIFF interp_cclause C = interp_cclause (delete_literals x C)` by
+    fs[interp_cclause_delete_literals]>>
+  `wf_clause x` by
+    (fs[wf_fml_def,values_def]>>
+    metis_tac[])>>
+  `MEM h' (delete_literals x C)` by fs[]>>
+  `-h' ≠ 0` by
+    (fs[wf_clause_def,delete_literals_def,MEM_FILTER]>>
+    metis_tac[])>>
+  first_x_assum drule>>
+  disch_then(qspecl_then [`-h'::C`,`D`] mp_tac)>>simp[]>>
+  impl_tac >-
+    (fs[wf_clause_def]>>
+    intLib.ARITH_TAC)>>
   strip_tac>>
-  TOP_CASE_TAC>>
-  TOP_CASE_TAC
-  >-
-    (strip_tac>>first_x_assum drule>> simp[]>>
-    reverse (rw[]) >- metis_tac[]>>
-    match_mp_tac (GEN_ALL tautology_asymmetric_tautology)>>
-    qpat_x_assum`wf_clause C` assume_tac>>
-    drule find_tauto_correct>>
-    disch_then drule>>strip_tac>>
-    qexists_tac`interp_lit l`>>simp[]>>
-    `-p ≠ 0` by fs[]>>
-    simp[interp_cclause_sorted_delete]>>
-    simp[interp_cclause_def]>>
-    `l ≠ 0 ∧ -l ≠ 0` by
-      (fs[wf_clause_def]>>
-      metis_tac[])>>
-    simp[negate_literal_interp_lit]>>
-    rw[]
-    >-
-      (DISJ2_TAC>>fs[delete_literal_def]>>
-      metis_tac[interp_lit_eq])
-    >> metis_tac[])
-  >>
-  (* 5.3 *)
-  reverse (rw[]>>fs[]) >- metis_tac[]
-  >>
-  last_x_assum kall_tac>> fs[]>>
-  drule is_AT_imp_asymmetric_tautology>>
-  `wf_clause (sorted_delete (-p) Ci)` by
-    metis_tac[wf_clause_sorted_delete]>>
-  `wf_clause (sorted_union C (sorted_delete (-p) Ci))` by
-    metis_tac[wf_clause_sorted_union]>>
-  disch_then drule>>
-  disch_then drule>>
-  fs[]>>
-  metis_tac[interp_cclause_sorted_union]
+  qexists_tac`E ∪ interp_cclause [-h']`>> simp[]>>
+  simp[Once interp_cclause_cons,UNION_ASSOC]>>
+  rw[sat_implies_def]>>fs[sat_implies_def]>>
+  qpat_x_assum` _ D = _` SUBST_ALL_TAC>>
+  first_x_assum drule>>
+  strip_tac>>
+  fs[satisfies_INSERT]>>
+  `satisfies_clause w (interp_cclause x)` by
+    (fs[satisfies_def,interp_def,values_def]>>
+    metis_tac[])>>
+  CCONTR_TAC >> fs[]>>
+  `interp_cclause x DIFF interp_cclause C = interp_cclause [h']` by
+    fs[]>>
+  `satisfies_clause w (interp_cclause [h'])` by
+    metis_tac[satisfies_clause_DIFF]>>
+  fs[satisfies_clause_union]>>
+  qpat_x_assum`h' ≠ 0` mp_tac>>
+  rpt (qpat_x_assum`satisfies_clause w _` mp_tac)>>
+  PURE_REWRITE_TAC [Once interp_cclause_cons,Once satisfies_clause_union]>>
+  strip_tac>>
+  pop_assum mp_tac>>
+  rpt( pop_assum kall_tac)>>
+  rw[interp_cclause_def]>>
+  fs[satisfies_clause_def]>>
+  metis_tac[negate_literal_interp_lit,satisfies_literal_exclusive]
 QED
 
-Theorem is_RAT_imp_resolution_asymmetric_tautology:
-  ∀fml p C i0 ik.
-  wf_fml fml ∧ wf_clause C ∧ (p ≠ 0 ⇒ MEM p C) ⇒
-  is_RAT fml p C i0 ik ⇒
-  satisfiable (interp fml) ⇒ satisfiable ((interp_cclause C) INSERT interp fml)
+Theorem check_overlap_eq:
+  ∀D.
+  check_overlap C D  ⇔
+  ∃x. MEM x C ∧ MEM x D
 Proof
-  rw[is_RAT_def]>>
-  ntac 2 (pop_assum mp_tac)>> ntac 2 TOP_CASE_TAC>>fs[]
-  >-
-    (drule is_AT_imp_asymmetric_tautology>>
-    rpt (disch_then drule)>>
-    metis_tac[asymmetric_tautology_satisfiable]) >>
-  drule is_AT_imp_sat_preserving>>
-  rpt (disch_then drule)>>
-  rw[]>>
-  `EVERY wf_clause (MAP SND (toAList fml))` by
-    fs[EVERY_MEM,MEM_MAP,EXISTS_PROD,MEM_toAList,wf_fml_def,values_def]>>
-  drule is_RAT_aux_imp>>
-  rpt (disch_then drule)>>
-  simp[MEM_toAList]>>
+  Induct>>rw[check_overlap_def]>>
+  metis_tac[]
+QED
+
+(* Some sanity checks:
+  is_AT in INL() case is independent of ordering
+*)
+
+(* TODO: these antitone theorems can be stated more precisely *)
+Theorem delete_literals_antitone:
+  ∀ls.
+  (∀x. MEM x D ⇒ MEM x C) ⇒
+  (∀y. MEM y (delete_literals ls C) ⇒ MEM y (delete_literals ls D))
+Proof
+  rw[delete_literals_def,MEM_FILTER]>>
+  metis_tac[]
+QED
+
+Theorem delete_literals_antitone_LENGTH:
+  ∀ls.
+  (∀x. MEM x D ⇒ MEM x C) ⇒
+  LENGTH (delete_literals ls C) ≤ LENGTH (delete_literals ls D)
+Proof
+  rw[delete_literals_def]>>
+  match_mp_tac LENGTH_FILTER_LEQ_MONO>>
+  metis_tac[]
+QED
+
+Theorem is_AT_INL_reorder:
+  ∀is C D.
+  (∀x. MEM x D ⇒ MEM x C) /\ is_AT fml is D = SOME (INL ()) ⇒
+  is_AT fml is C = SOME (INL ())
+Proof
+  Induct>> rw[is_AT_def]>>
+  TOP_CASE_TAC>>fs[]>>
+  TOP_CASE_TAC>>fs[]>>
+  TOP_CASE_TAC>>fs[]
+  >- (
+    drule delete_literals_antitone_LENGTH>>
+    disch_then(qspec_then`x` assume_tac)>>rfs[]>>
+    every_case_tac>>fs[]>>
+    `h'=h''` by
+      (drule delete_literals_antitone>>
+      disch_then(qspec_then`x` assume_tac)>>rfs[])>>
+    rw[]>>
+    metis_tac[MEM])
+  >>
+  drule delete_literals_antitone_LENGTH>>
+  disch_then(qspec_then`x` assume_tac)>>rfs[]>>
+  every_case_tac>>fs[]
+QED
+
+(* Converse is true assuming p and ¬p are not both in Ci *)
+Theorem check_RAT_imp_check_PR:
+  check_RAT fml p C ik (i,Ci) ==>
+  check_PR fml p C [p] ik (i,Ci)
+Proof
+  rw[check_RAT_def,check_PR_def]>>
+  fs[flip_def,overlap_assignment_def]>>
+  every_case_tac>>fs[]>>
+  fs[check_overlap_eq]>>
+  rw[]>>fs[]>>
+  match_mp_tac is_AT_INL_reorder>>
+  HINT_EXISTS_TAC>>fs[]>>
+  simp[MAP_MAP_o,o_DEF]>>
+  rw[delete_literals_def,MEM_FILTER]>>
+  metis_tac[]
+QED
+
+(*
+  The witnessing assignment is
+    interp_cclause w ∪ (IMAGE negate_literal (interp_cclause C DIFF interp_cclause w))
+*)
+Theorem DIFF_ID:
+  A DIFF B = A ⇔ A ∩ B = {}
+Proof
+  rw[EXTENSION]>>
+  metis_tac[]
+QED
+
+Theorem INTER_UNION_EMPTY:
+  A ∩ (B ∪ C) = {} ⇔
+  A ∩ B = {} ∧ A ∩ C = {}
+Proof
+  rw[EXTENSION]>>
+  metis_tac[]
+QED
+
+Theorem MEM_overlap_assignment:
+  MEM x (overlap_assignment w C) =
+  (MEM x w ∨ MEM (-x) C ∧ ¬MEM (-x) w)
+Proof
+  rw[overlap_assignment_def,flip_def,MEM_MAP,delete_literals_def,MEM_FILTER]>>
+  Cases_on`MEM x w`>>simp[]>>
+  rw[EQ_IMP_THM]>>fs[]>>
+  qexists_tac`-x`>> simp[]
+QED
+
+Theorem interp_cclause_flip:
+  interp_cclause (flip C) = IMAGE negate_literal (interp_cclause C)
+Proof
+  rw[interp_cclause_def,flip_def,EXTENSION,MEM_MAP,EQ_IMP_THM]
+  >- (
+    qexists_tac`interp_lit i`>>
+    `i ≠ 0` by fs[]>>
+    simp[negate_literal_interp_lit]>>
+    metis_tac[])
+  >>
+  qexists_tac`-x''`>>
+  simp[negate_literal_interp_lit]
+QED
+
+Theorem check_PR_sat_implies:
+  check_PR fml p C w ik (i,Ci) ∧ Ci ∈ values fml ∧
+  wf_fml fml ∧ wf_clause C ∧ consistent_par (interp_cclause C) ⇒
+  sat_implies (par (IMAGE negate_literal (interp_cclause C)) (interp fml))
+    (par
+      (interp_cclause w ∪ (IMAGE negate_literal (interp_cclause C DIFF interp_cclause w)))
+      {interp_cclause Ci})
+Proof
+  simp[check_PR_def]>>
+  reverse (Cases_on`check_overlap Ci (flip w)`)
+  >- (
+    (* 5.1: Ci not touched by w *)
+    rw[sat_implies_def,par_def,satisfies_def]>>
+    simp[DIFF_UNION]>>
+    `interp_cclause Ci DIFF IMAGE negate_literal (interp_cclause w) = interp_cclause Ci` by
+      (simp[DIFF_ID,interp_cclause_def,EXTENSION]>>
+      rw[]>>CCONTR_TAC>>fs[check_overlap_eq,flip_def,MEM_MAP]>>
+      metis_tac[interp_lit_eq,negate_literal_interp_lit])>>
+    fs[INTER_UNION_EMPTY,IMAGE_IMAGE]>>
+    first_x_assum match_mp_tac>>
+    simp[PULL_EXISTS,interp_def]>>
+    fs[EXTENSION]>>
+    metis_tac[]) >>
+  simp[]>>
   strip_tac>>
-  `resolution_asymmetric_tautology (interp fml) (interp_cclause y)` by
-    (simp[resolution_asymmetric_tautology_def]>>
-    DISJ2_TAC>>
-    qexists_tac`interp_lit p`>>fs[interp_def,PULL_EXISTS,values_def]>>
-    CONJ_TAC >-
-      (DISJ2_TAC>>simp[interp_cclause_def])>>
-    rw[negate_literal_interp_lit]>>
-    `wf_clause x` by
-      (fs[wf_fml_def,values_def]>>
+  `wf_clause Ci` by
+    fs[wf_fml_def]>>
+  Cases_on`lookup i ik`>>
+  simp[]
+  >- (
+    (* 5.2.1: Ci already satisfied by w *)
+    rw[sat_implies_def,par_def,satisfies_def]>>
+    fs[INTER_UNION_EMPTY,check_overlap_eq]>>
+    `interp_lit x' ∈ interp_cclause Ci ∩ interp_cclause w` by
+      (fs[wf_clause_def]>>
+      simp[interp_cclause_def]>>
       metis_tac[])>>
-    first_x_assum drule>>
-    impl_tac >-
-      (fs[interp_cclause_def]>>
-      `-p = x'` by metis_tac[interp_lit_eq]>>
-      metis_tac[sorted_mem_correct])>>
-    simp[interp_cclause_sorted_delete])>>
-  drule resolution_asymmetric_tautology_satisfiable>>
+    fs[EXTENSION]>>
+    metis_tac[])>>
+  Cases_on`x`>>fs[]
+  >- (
+    (* 5.2.2: Ci already satisfied by w ∪ alpha+ *)
+    rw[sat_implies_def,par_def,satisfies_def]>>
+    fs[INTER_UNION_EMPTY,check_overlap_eq]>>
+    qmatch_asmsub_abbrev_tac `A = {}`>>
+    qsuff_tac`interp_lit x' ∈ A`
+    >- fs[EXTENSION]>>
+    simp[Abbr`A`]>>
+    CONJ_ASM1_TAC >- (
+      fs[interp_cclause_def,wf_clause_def]>>
+      metis_tac[])>>
+    fs[MEM_overlap_assignment]
+    >- (
+      `interp_lit x' ∈ interp_cclause w` by
+        (fs[wf_clause_def]>>
+        simp[interp_cclause_def]>>
+        metis_tac[])>>
+      fs[EXTENSION]>>
+      metis_tac[])>>
+    qexists_tac`interp_lit (-x')`>>
+    `-x' ≠ 0` by (fs[wf_clause_def] >> metis_tac[])>>
+    simp[negate_literal_interp_lit]>>
+    fs[wf_clause_def,interp_cclause_def]>>
+    metis_tac[interp_lit_eq])>>
+  (* 5.3 *)
+  rw[sat_implies_def]>>
+  simp[satisfies_def,par_def]>>
+  strip_tac>>
+  drule is_AT_imp_asymmetric_tautology>>
+  qmatch_asmsub_abbrev_tac`is_AT _ _ D = SOME _`>>
+  disch_then(qspecl_then[`h::t`,`D`] mp_tac)>>
+  simp[]>>
+  impl_tac >-
+    (simp[Abbr`D`,delete_literals_def]>>
+    fs[wf_clause_def,MEM_FILTER])>>
+  simp[Abbr`D`,interp_cclause_append]>>
+  simp[overlap_assignment_def,interp_cclause_delete_literals,interp_cclause_flip,interp_cclause_append,IMAGE_IMAGE]>>
+  strip_tac>>
+  drule asymmetric_tautology_union_clause2 >>
+  disch_then drule>>
+  impl_tac >-
+    (fs[EXTENSION]>> metis_tac[])>>
+  strip_tac>>
+  drule asymmetric_tautology_satisfies>>
+  disch_then drule>>
+  simp[satisfies_INSERT,interp_cclause_delete_literals,interp_cclause_flip]>>
+  simp[overlap_assignment_def,interp_cclause_append,interp_cclause_flip,IMAGE_IMAGE,interp_cclause_delete_literals]>>
+  qmatch_goalsub_abbrev_tac`_ _ A ==> _ _ B`>>
+  qsuff_tac`A=B` >- fs[]>>
+  unabbrev_all_tac>>fs[EXTENSION]>>
+  metis_tac[]
+QED
+
+Theorem redundant_sat_implies:
+  sat_implies (D INSERT fml) (C INSERT fml) ∧
+  redundant fml D
+  ⇒
+  redundant fml C
+Proof
+  rw[sat_implies_def,redundant_def]>>
+  fs[]>>
   metis_tac[satisfiable_def]
+QED
+
+Theorem sat_implies_values:
+  (∀C. C ∈ values fml ⇒ sat_implies A (par w {interp_cclause C})) ⇒
+  sat_implies A (par w (interp fml))
+Proof
+  rw[sat_implies_def,satisfies_def,interp_def,par_def]>>
+  metis_tac[]
+QED
+
+Theorem consistent_par_union:
+  consistent_par A ∧
+  consistent_par B ∧
+  A ∩ B = {} ⇒
+  consistent_par (A ∪ IMAGE negate_literal B)
+Proof
+  rw[consistent_par_def,IMAGE_IMAGE]>>
+  simp[INTER_UNION_EMPTY,INTER_UNION]>>
+  fs[EXTENSION]>>
+  metis_tac[negate_literal_11]
+QED
+
+Theorem consistent_par_DIFF:
+  consistent_par A ⇒ consistent_par (A DIFF B)
+Proof
+  rw[consistent_par_def,EXTENSION]>>
+  metis_tac[]
+QED
+
+Theorem check_overlap_flip_consistent_par:
+  ¬check_overlap x (flip x) ⇒
+  consistent_par (interp_cclause x)
+Proof
+  rw[consistent_par_def,interp_cclause_def,EXTENSION,check_overlap_eq,flip_def,MEM_MAP]>>
+  CCONTR_TAC>>fs[]>>
+  rename1 `MEM A x`>>
+  qpat_x_assum`MEM _ _` mp_tac>>
+  rename1 `MEM B x`>>
+  first_x_assum(qspec_then`A` assume_tac)>>rfs[]>>
+  first_x_assum(qspec_then`B` assume_tac)>>rfs[]>>
+  `B ≠ -A` by intLib.ARITH_TAC>>
+  metis_tac[interp_lit_eq,negate_literal_interp_lit]
+QED
+
+Theorem is_PR_redundant:
+  wf_clause C ∧ wf_fml fml ∧
+  (p ≠ 0 ⇒ MEM p C ∧
+    case w of SOME ww =>
+      MEM p ww
+    | NONE => T) ∧
+  is_PR fml p C w i0 ik  ⇒
+  redundant (interp fml) (interp_cclause C)
+Proof
+  simp[is_PR_def]>>
+  strip_tac>>
+  pop_assum mp_tac>>
+  ntac 2 (TOP_CASE_TAC>>fs[])
+  >-
+    metis_tac[is_AT_imp_asymmetric_tautology,asymmetric_tautology_redundant]
+  >>
+  strip_tac>>
+  drule is_AT_imp_sat_implies>>
+  disch_then drule>>
+  disch_then drule>>
+  strip_tac>>
+  drule redundant_sat_implies>>
+  disch_then match_mp_tac>>
+  reverse (Cases_on`consistent_par (E ∪ interp_cclause C)`)
+  >-
+    metis_tac[not_consistent_par_redundant]>>
+  reverse (Cases_on`w`)>>fs[]
+  >- (
+    (* PR *)
+    match_mp_tac par_redundant>>
+    qexists_tac`(interp_cclause x ∪
+               IMAGE negate_literal (E ∪ interp_cclause C DIFF interp_cclause x))`>>
+               simp[]>>
+    CONJ_TAC >- (
+      match_mp_tac consistent_par_union>>
+      rw[]
+      >-
+        metis_tac[check_overlap_flip_consistent_par]
+      >-
+        metis_tac[consistent_par_DIFF]
+      >>
+        simp[EXTENSION]>>
+        metis_tac[])>>
+    CONJ_TAC >- (
+      `interp_lit p ∈ interp_cclause x ∧ interp_lit p ∈ interp_cclause C` by
+        fs[interp_cclause_def]>>
+      simp[EXTENSION]>>
+      metis_tac[])>>
+    match_mp_tac sat_implies_values>>
+    rw[values_def]>>fs[EVERY_MEM,MEM_toAList,FORALL_PROD]>>
+    first_x_assum drule>>
+    strip_tac>>
+    drule check_PR_sat_implies>>
+    simp[]>>
+    impl_tac >-
+      (fs[values_def]>>
+      metis_tac[])>>
+    simp[])
+  >>
+    (* RAT *)
+    match_mp_tac par_redundant>>
+    qexists_tac`({interp_lit p} ∪
+               IMAGE negate_literal (E ∪ interp_cclause C DIFF {interp_lit p}))`>>
+               simp[]>>
+    CONJ_TAC >- (
+      match_mp_tac consistent_par_union>>
+      rw[]
+      >-
+        metis_tac[consistent_par_DIFF]
+      >>
+        simp[EXTENSION]>>
+        metis_tac[])>>
+    CONJ_TAC >- (
+      `interp_lit p ∈ interp_cclause C` by
+        fs[interp_cclause_def]>>
+      simp[EXTENSION]>>
+      metis_tac[])>>
+    match_mp_tac sat_implies_values>>
+    rw[values_def]>>fs[EVERY_MEM,MEM_toAList,FORALL_PROD]>>
+    first_x_assum drule>>
+    strip_tac>>
+    drule check_RAT_eq_check_PR>>
+    rw[]>>
+    drule check_PR_sat_implies>>
+    simp[]>>
+    impl_tac >-
+      (fs[values_def]>>
+      metis_tac[])>>
+    simp[interp_cclause_def]
 QED
 
 (* Deletion preserves sat: if C is satisfiable, then deleting clauses from C keeps satisfiability *)
@@ -1262,9 +795,8 @@ QED
 
 Theorem delete_clauses_sound:
   ∀l fml. satisfiable (interp fml) ⇒
-  satisfiable (interp (list_delete l fml))
+  satisfiable (interp (FOLDL (λa b. delete b a) fml l))
 Proof
-  simp[list_delete_def]>>
   Induct>>simp[]>>
   rw[]>>metis_tac[delete_preserves_satisfiable]
 QED
@@ -1280,6 +812,7 @@ QED
 Theorem check_lrat_step_sound:
   ∀lrat fml fml'.
   wf_fml fml ∧
+  (* TODO: should assume that PR never has 0s in the clause and prove in parser *)
   check_lrat_step lrat fml = SOME fml' ⇒
   (satisfiable (interp fml) ⇒ satisfiable (interp fml'))
 Proof
@@ -1290,30 +823,28 @@ Proof
     (simp[]>>
     metis_tac[delete_clauses_sound])
   >>
-  qmatch_goalsub_abbrev_tac`is_RAT _ _ ls _ _`>>
-  `wf_clause ls` by
-    (fs[wf_clause_def,Abbr`ls`,QSORT_MEM,MEM_FILTER]>>
-    match_mp_tac QSORT_SORTED>>
-    fs[transitive_def,total_def]>>
-    intLib.ARITH_TAC)>>
-  strip_tac>>
-  drule is_RAT_imp_resolution_asymmetric_tautology>>
-  rpt (disch_then drule)>>
-  simp[Once CONJ_COMM]>>
-  disch_then drule>>
-  impl_tac>-
-    (every_case_tac>>simp[Abbr`ls`,QSORT_MEM])>>
-  rveq>>fs[]>>
+  rw[]>>
+  `redundant (interp fml) (interp_cclause l)` by
+    (match_mp_tac (GEN_ALL is_PR_redundant)>>
+    simp[]>>
+    PURE_REWRITE_TAC[Once CONJ_ASSOC]>>
+    PURE_REWRITE_TAC[Once CONJ_COMM]>>
+    asm_exists_tac>>
+    simp[]>>
+    Cases_on`l`>>simp[]>>
+    cheat)>>
+  fs[redundant_def]>>
+  first_x_assum drule>>
   match_mp_tac satisfiable_SUBSET>>
-  metis_tac[interp_insert]
+  simp[interp_insert]
 QED
 
 Theorem wf_fml_delete_clauses:
   ∀l fml.
   wf_fml fml ⇒
-  wf_fml (list_delete l fml)
+  wf_fml (FOLDL (λa b. delete b a) fml l)
 Proof
-  simp[list_delete_def,FOLDL_FOLDR_REVERSE]>>
+  simp[FOLDL_FOLDR_REVERSE]>>
   strip_tac>>
   qabbrev_tac`ll= REVERSE l`>>
   pop_assum kall_tac>>
@@ -1350,10 +881,7 @@ Proof
   strip_tac>>
   rveq>>fs[]>>
   match_mp_tac wf_fml_insert>>fs[]>>
-  simp[wf_clause_def,QSORT_MEM,MEM_FILTER]>>
-  match_mp_tac QSORT_SORTED>>
-  fs[transitive_def,total_def]>>
-  intLib.ARITH_TAC
+  cheat
 QED
 
 (* The main theorem *)
@@ -1370,11 +898,12 @@ Proof
   strip_tac>>
   drule check_lrat_step_sound>>
   rpt (disch_then drule)>>
-  drule check_lrat_step_wf_fml>>
+  cheat
+  (*drule check_lrat_step_wf_fml>>
   rpt (disch_then drule)>>
   strip_tac>>
   strip_tac>>
-  first_x_assum(qspec_then`x` mp_tac)>> simp[]
+  first_x_assum(qspec_then`x` mp_tac)>> simp[] *)
 QED
 
 Theorem is_unsat_sound:
@@ -1404,27 +933,24 @@ Proof
 QED
 
 (* Try on an example
-val fml = rconc (EVAL ``insert 1 [ 1;  2; -3] (
-  insert 2 [-1; -2;  3] (
-  insert 3 [ 2;  3; -4] (
-  insert 4 [-2; -3;  4] (
-  insert 5 [-1; -3; -4] (
-  insert 6 [ 1;  3;  4] (
-  insert 7 [-1;  2;  4] (
-  insert 8 [ (1:int); -2; -4] LN))))))) :ccnf``)
+val fml = rconc (EVAL
+``insert 1 [ -3;  1;  2] (
+  insert 2 [ -2; -1;  3] (
+  insert 3 [ -4;  2;  3] (
+  insert 4 [ -3; -2;  4] (
+  insert 5 [ -4; -3; -1] (
+  insert 6 [  1;  3;  4] (
+  insert 7 [ -1;  2;  4] (
+  insert 8 [ -4; -2; (1:int)] LN))))))) :ccnf``)
 
 val lrat =
 ``[
   Delete [];
-  RAT 9 [-1] [] (insert 1 [5;7] (insert 6 [2;7] (insert 8 [5;2] LN)));
-  Delete [7;5;2] ;
-  RAT 10 [2] [9;1;6;3] LN;
-  Delete [1;3;0] ;
-  RAT 12 [] [9;10;8;4;6] LN
+  PR 9 [-1] NONE [] (insert 1 [5;7] (insert 6 [2;7] (insert 8 [5;2] LN)));
 ]``;
 
-  (* result contains the empty clause *)
-val res = EVAL``check_lrat_unsat ^(lrat) ^(fml)``
- *)
+(* result contains the empty clause *)
+  val res = EVAL``check_lrat ^(lrat) ^(fml)``
+*)
 
 val _ = export_theory ();
